tmp

code/experimental/rsa/Division.fst
@@ -3,8 +3,8 @@ module Division
 open FStar.HyperStack.All
 open FStar.Buffer
 open FStar.Int.Cast
-open Convert
 
+open Convert
 open Shift
 open Comparison
 open Addition
@@ -14,49 +14,67 @@ module U64 = FStar.UInt64
 
 type bignum = buffer FStar.UInt64.t
 
-let bn_bits2 = 64ul
-
 val remainder_loop:
-    rLen:U32.t -> modLen:U32.t -> resLen:U32.t ->
-    r_i:bignum{length r_i = U32.v rLen} -> mod:bignum{length mod = U32.v modLen} ->
-    count:U32.t -> res:bignum{length res = U32.v resLen} -> Stack unit
+    rLen:U32.t{U32.v rLen > 0} ->
+    modLen:U32.t{U32.v modLen > 0 /\ U32.v modLen = U32.v rLen} ->
+    resLen:U32.t{U32.v resLen > 0 /\ U32.v resLen <= U32.v modLen} ->
+    r_i:bignum{length r_i = U32.v rLen} ->
+    mod:bignum{length mod = U32.v modLen /\ disjoint r_i mod} ->
+    count:U32.t ->
+    res:bignum{length res = U32.v resLen /\ disjoint res r_i} -> 
+    Stack unit
     (requires (fun h -> live h r_i /\ live h mod /\ live h res))
 	(ensures (fun h0 _ h1 -> live h0 r_i /\ live h0 mod /\  live h0 res /\ 
-        live h1 res /\ modifies_1 res h0 h1))
+        live h1 r_i /\ live h1 mod /\ live h1 res /\ 
+         modifies_1 mod h0 h1 /\ modifies_1 res h0 h1 /\ modifies_1 r_i h0 h1))
+
+#set-options "--z3rlimit 50 --max_fuel 2"
+
 let rec remainder_loop rLen modLen resLen r_i mod count res =
     push_frame();
-    let isSet = if U64.(mod.(U32.(modLen -^ 1ul)) =^ 1uL) then 1ul else 0ul in
-    let mod1Len = U32.(modLen -^ isSet) in
-    let mod1 = create 0uL mod1Len in
+    let mod1 = create 0uL modLen in
     let tmp = create 0uL rLen in
     (if U32.(count >^ 0ul) then
-       (rshift1 modLen mod mod1;
-        if not (isMore modLen rLen mod r_i) then
-		   (sub rLen modLen r_i mod tmp; blit tmp 0ul r_i 0ul rLen;
-		    remainder_loop rLen mod1Len resLen r_i mod1 U32.(count -^ 1ul) res)
-	    else remainder_loop rLen mod1Len resLen r_i mod1 U32.(count -^ 1ul) res)
-    else
-        let len = if U32.(resLen >^ rLen) then rLen else resLen in
-        blit r_i 0ul res 0ul len);
+        begin
+        rshift1 modLen mod mod1;
+        let tmp_b = isMore modLen rLen mod r_i in
+        (if not tmp_b then
+            sub rLen modLen r_i mod tmp;
+            blit tmp 0ul r_i 0ul rLen);
+        remainder_loop rLen modLen resLen r_i mod1 U32.(count -^ 1ul) res
+        end
+    else blit r_i 0ul res 0ul resLen);
     pop_frame()
 
 (* res = a % mod *)
 val remainder:
-    aBits:U32.t -> modBits:U32.t{U32.(modBits <^ aBits)} -> resLen:U32.t ->
+    aBits:U32.t{U32.v aBits > 0} ->
+    modBits:U32.t{U32.v modBits > 0 /\ U32.v aBits >= U32.v modBits} ->
+    resLen:U32.t{U32.v resLen > 0} ->
     a:bignum{length a = U32.v (bits_to_bn aBits)} ->
-    mod:bignum{length mod = U32.v (bits_to_bn modBits)} ->
-    res:bignum{length res = U32.v resLen} -> Stack unit
+    mod:bignum{length mod = U32.v (bits_to_bn modBits) /\ length mod <= length a /\ disjoint a mod} ->
+    res:bignum{length res = U32.v resLen /\ length res <= length mod /\ disjoint a res} -> Stack unit
 	(requires (fun h -> live h a /\ live h mod /\ live h res))
-	(ensures (fun h0 _ h1 -> live h0 a /\ live h0 mod /\  live h0 res /\ 
-        live h1 res /\ modifies_1 res h0 h1))
+	(ensures (fun h0 _ h1 -> live h0 a /\ live h0 mod /\  live h0 res /\
+        live h1 a /\ live h1 mod /\ live h1 res /\ modifies_1 res h0 h1))
+
+#set-options "--z3rlimit 50"
+
 let remainder aBits modBits resLen a mod res =
     push_frame();
     let aLen = bits_to_bn aBits in
+    assert(length a = U32.v (bits_to_bn aBits));
     let modLen = bits_to_bn modBits in
+    assert(length mod = U32.v (bits_to_bn modBits));
     let k = U32.(aBits -^ modBits) in
-    let modk = U32.(k /^ bn_bits2) in
-    let mod1Len = U32.(modLen +^ modk) in
+    let modk = U32.(k /^ 64ul) in
+    assume(U32.v modLen + U32.v modk + 1 < pow2 32);
+    let mod1Len = U32.(modLen +^ modk +^ 1ul) in
+    let a1Len = U32.(aLen +^ 1ul) in
+    assert(U32.v mod1Len = U32.v a1Len);
     let mod1 = create 0uL mod1Len in
     lshift modLen mod k mod1;
-    remainder_loop aLen mod1Len resLen a mod1 k res;
+    let r_0 = create 0uL a1Len in
+    lshift aLen a 64ul r_0;
+    remainder_loop a1Len mod1Len resLen r_0 mod1 k res;
     pop_frame()
