code/experimental/rsa/Shift.fst
@@ -9,9 +9,7 @@ module U64 = FStar.UInt64
 
 type bignum = buffer FStar.UInt64.t
 
-let bn_bits2 = 64ul
 let bn_tbit = 0x8000000000000000uL
-let bn_mask2 = 0xffffffffffffffffuL
 
 val lshift_loop:
     a:bignum{length a > 0} ->
@@ -31,15 +29,16 @@ let rec lshift_loop a count nw lb res =
         let t1 = a.(count) in
         let rb = U32.(64ul -^ lb) in
         assert(0 < U32.v rb /\ U32.v rb < 64);
-        res.(ind) <- U64.(tmp |^ (U64.(t1 >>^ rb) &^ bn_mask2));
-        res.(U32.(ind -^ 1ul)) <- U64.((t1 <<^ lb) &^ bn_mask2);
+        res.(ind) <- U64.(tmp |^ U64.(t1 >>^ rb));
+        res.(U32.(ind -^ 1ul)) <- U64.(t1 <<^ lb);
         lshift_loop a count nw lb res
     else ()
 
 (* res = a << n *)
 val lshift:
     aLen:U32.t{U32.v aLen > 0} ->
-    a:bignum{length a = U32.v aLen} -> nCount:U32.t{U32.v nCount> 0} ->
+    a:bignum{length a = U32.v aLen} -> 
+    nCount:U32.t ->
     res:bignum{length res = U32.v aLen + U32.v nCount / 64 + 1 /\ disjoint a res} -> 
     Stack unit
 	(requires (fun h -> live h a /\ live h res))
@@ -48,7 +47,7 @@ val lshift:
 
 let lshift aLen a nCount res =
     let nw = U32.(nCount/^ 64ul) in
-    let resLen = U32.(aLen +^ nw) in
+    let resLen = U32.(aLen +^ nw +^ 1ul) in
     let lb = U32.(nCount %^ 64ul) in
     (if U32.(lb =^ 0ul) then
         blit a 0ul res nw aLen
@@ -69,7 +68,7 @@ let rec rshift1_loop a carry ind res =
     if U32.(ind >^ 0ul) then
         let ind = U32.(ind -^ 1ul) in
         let tmp = a.(ind) in
-        res.(ind) <- U64.(((tmp >>^ 1ul) &^ bn_mask2) |^ carry);
+        res.(ind) <- U64.((tmp >>^ 1ul) |^ carry);
         let carry = if U64.((tmp &^ 1uL) =^ 1uL) then bn_tbit else 0uL in
         rshift1_loop a carry ind res
     else ()
