code/experimental/rsa/Comparison.fst
@@ -11,11 +11,13 @@ module I32 = FStar.Int32
 type bignum = buffer FStar.UInt64.t
 
 val isMore_loop:
-    a:bignum -> b:bignum{length b = length a} -> 
+    a:bignum -> 
+    b:bignum{length b = length a} -> 
     count:U32.t{U32.v count <= length a} -> Stack bool
     (requires (fun h -> live h a /\ live h b))
 	(ensures (fun h0 _ h1 -> live h0 a /\ live h0 b
          /\ live h1 a /\ live h1 b))
+
 let rec isMore_loop a b count =
     if U32.(count >^ 0ul) then
         let count = U32.(count -^ 1ul) in
@@ -28,12 +30,14 @@ let rec isMore_loop a b count =
 
 (* if a > b then true else false *)
 val isMore:
-    aLen:U32.t -> bLen:U32.t ->
+    aLen:U32.t{U32.v aLen > 0} -> 
+    bLen:U32.t{U32.v bLen > 0} ->
     a:bignum{length a = U32.v aLen} -> 
-    b:bignum{length b = U32.v bLen} -> Stack bool
+    b:bignum{length b = U32.v bLen /\ disjoint a b} -> Stack bool
     (requires (fun h -> live h a /\ live h b))
 	(ensures (fun h0 _ h1 -> live h0 a /\ live h0 b 
         /\ live h1 a /\ live h1 b))
+        
 let isMore aLen bLen a b =
     if U32.(aLen >^ bLen) then true
     else if U32.(aLen <^ bLen) then false
